Weidenbach_Book/IsaSAT/IsaSAT_Decide_LLVM.thy
@@ -1,15 +1,25 @@
 theory IsaSAT_Decide_LLVM
   imports IsaSAT_Decide IsaSAT_VMTF_State_LLVM IsaSAT_Setup_LLVM IsaSAT_Rephase_State_LLVM
 begin
-
+lemma decide_lit_wl_heur_alt_def:
+  \<open>decide_lit_wl_heur = (\<lambda>L' S. do {
+      let (M, S) = extract_trail_wl_heur S;
+      let (stats, S) = extract_stats_wl_heur S;
+      ASSERT(isa_length_trail_pre M);
+      let j = isa_length_trail M;
+      let S = update_literals_to_update_wl_heur j S;
+      ASSERT(cons_trail_Decided_tr_pre (L', M));
+      let M = cons_trail_Decided_tr L' M;
+      let S = update_trail_wl_heur M S;
+      let S = update_stats_wl_heur stats S;
+        RETURN S})\<close>
+   by (auto simp: decide_lit_wl_heur_def state_extractors split: isasat_int.splits intro!: ext)
 
 sepref_def decide_lit_wl_fast_code
   is \<open>uncurry decide_lit_wl_heur\<close>
   :: \<open>unat_lit_assn\<^sup>k *\<^sub>a isasat_bounded_assn\<^sup>d \<rightarrow>\<^sub>a isasat_bounded_assn\<close>
   supply [[goals_limit=1]]
-  unfolding decide_lit_wl_heur_def isasat_bounded_assn_def
-  (*supply hn_case_prod'[sepref_comb_rules del]*)
-  unfolding fold_tuple_optimizations
+  unfolding decide_lit_wl_heur_alt_def
   by sepref
 
 
@@ -39,376 +49,67 @@ sepref_def isa_vmtf_find_next_undef_upd_code is
   unfolding isa_vmtf_find_next_undef_upd_def
   by sepref
 
+lemma find_unassigned_lit_wl_D_heur2_alt_def:
+  \<open>find_unassigned_lit_wl_D_heur2 = (\<lambda>S. do {
+    let (M, S) = extract_trail_wl_heur S;
+    let (vm, S) = extract_vmtf_wl_heur S;
+    let (heur, S) = extract_heur_wl_heur S;
+      ((M, vm), L) \<leftarrow> isa_vmtf_find_next_undef_upd M vm;
+      RETURN (update_heur_wl_heur (set_fully_propagated_heur heur) (update_trail_wl_heur M (update_vmtf_wl_heur vm S)), L)
+    })\<close>
+   by (auto simp: find_unassigned_lit_wl_D_heur2_def state_extractors split: isasat_int.splits intro!: ext)
 sepref_register find_unassigned_lit_wl_D_heur2
 sepref_def find_unassigned_lit_wl_D_heur_impl
   is \<open>find_unassigned_lit_wl_D_heur2\<close>
   :: \<open>isasat_bounded_assn\<^sup>d \<rightarrow>\<^sub>a isasat_bounded_assn \<times>\<^sub>a atom.option_assn\<close>
-  unfolding find_unassigned_lit_wl_D_heur2_def isasat_bounded_assn_def
-    fold_tuple_optimizations
+  unfolding find_unassigned_lit_wl_D_heur2_alt_def
   by sepref
+
+sepref_definition get_next_phase_heur_stats_impl'
+  is \<open>uncurry2 (\<lambda>S C' D'. get_next_phase_heur C' D' S)\<close>
+  :: \<open>[uncurry2 (\<lambda>S C D. True)]\<^sub>a heuristic_assn\<^sup>k *\<^sub>a bool1_assn\<^sup>k *\<^sub>a atom_assn\<^sup>k \<rightarrow> bool1_assn\<close>
+  by sepref
+
+definition get_next_phase_st'_impl :: \<open>twl_st_wll_trail_fast2 \<Rightarrow> _\<close> where
+  \<open>get_next_phase_st'_impl = (\<lambda>N C D. read_heur_wl_heur_code (get_next_phase_heur_stats_impl C D) N)\<close>
+
+definition get_next_phase_st' :: \<open>_\<close> where
+  \<open>get_next_phase_st' N C D = (get_next_phase_st C D N)\<close>
+
+global_interpretation get_next_phase: read_heur_param_adder2 where
+  R = bool1_rel and
+  R' = atom_rel and
+  f' = \<open> \<lambda>C D S. get_next_phase_heur C D S\<close> and
+  f = \<open>\<lambda>C D S. get_next_phase_heur_stats_impl C D S\<close> and
+  x_assn = \<open>bool1_assn\<close> and
+  P = \<open>(\<lambda>_ _ _. True)\<close>
+  rewrites
+     \<open>(\<lambda>N C D. read_heur_wl_heur_code (get_next_phase_heur_stats_impl C D) N) = get_next_phase_st'_impl\<close> and
+     \<open>(\<lambda>N C D. read_heur_wl_heur (get_next_phase_heur C D) N) = get_next_phase_st'\<close>
+  apply unfold_locales
+  apply (rule get_next_phase_heur_stats_impl'.refine[unfolded get_next_phase_heur_stats_impl'_def])
+  subgoal by (auto simp: get_next_phase_st'_impl_def)
+  subgoal by (auto simp: read_all_wl_heur_def get_next_phase_st_def get_next_phase_st'_def split: isasat_int.splits
+    intro!: ext)
+  done
+
+lemmas [sepref_fr_rules] = get_next_phase.refine
+lemmas [unfolded inline_direct_return_node_case, llvm_code] =
+  get_next_phase_st'_impl_def[unfolded read_all_wl_heur_code_def]
 
 sepref_def get_next_phase_st_impl
   is \<open>uncurry2 get_next_phase_st\<close>
   :: \<open>bool1_assn\<^sup>k *\<^sub>a atom_assn\<^sup>k *\<^sub>a isasat_bounded_assn\<^sup>k \<rightarrow>\<^sub>a bool1_assn\<close>
-  unfolding get_next_phase_st_def isasat_bounded_assn_def fold_tuple_optimizations
+  unfolding get_next_phase_st'_def[symmetric]
   by sepref
-ML \<open>Sepref_Translate.gen_trans_step_tac\<close>
-thm sepref_fr_rules
-ML \<open>(Sepref_Translate.sepref_fr_rules.get @{context}) \<close>
-ML \<open>(Sepref_Translate.sepref_fr_rules.get @{context}) |> Tactic.build_net\<close>
-ML \<open>
-fun print start ctxt str _ = (print_tac ctxt (str ^ " " ^ (@{make_string} (Time.toMilliseconds (#elapsed (Timing.result start))))))
-
-    type phases_ctrl = {
-      trace: bool,            
-      trace_goals: bool,
-      int_res: bool,          
-      start: string option,   
-      stop: string option     
-    }
-    type phase = (unit -> string) * (Proof.context -> tactic') * int
-
-    local
-      fun ph_range (phases : phase list) start stop = let
-        fun find_phase name = let
-          val i = find_index (fn (n,_,_) => n()=name) phases
-          val _ = if i<0 then error ("No such phase: " ^ name) else ()
-        in
-          i
-        end
-
-        val i = case start of NONE => 0 | SOME n => find_phase n
-        val j = case stop of NONE => length phases - 1 | SOME n => find_phase n
-
-        val phases = take (j+1) phases |> drop i
-
-        val _ = case phases of [] => error "No phases selected, range is empty" | _ => ()
-      in
-        phases
-      end
-    in  
-  
-      fun PHASES' start phases (ctrl : phases_ctrl) ctxt = let
-        val phases = ph_range phases (#start ctrl) (#stop ctrl)
-        val phases = map (fn (n,tac,d) => (n,tac ctxt,d)) phases
-  
-        fun r [] _ st = Seq.single st
-          | r ((name,tac,d)::tacs) i st = let
-              val n = Thm.nprems_of st
-              val bailout_tac = if #int_res ctrl then all_tac else no_tac
-              fun trace_tac msg st = (if #trace ctrl then tracing msg else (); Seq.single st)
-              
-              val trace_goal_tac = if #trace_goals ctrl then print_tac ctxt "Proof state" else all_tac
-              
-              val trace_start_tac = trace_tac ("Phase " ^ (name ()))
-            in
-              K trace_goal_tac THEN' K trace_start_tac THEN' IF_EXGOAL (tac)
-              THEN_ELSE' (
-                fn i => fn st => 
-                  (* Bail out if a phase does not solve/create exactly the expected subgoals *)
-                  if Thm.nprems_of st = n+d then
-                    ((trace_tac ("  Done" ^ @{make_string} (Time.toMilliseconds (#elapsed (Timing.result start)))) THEN r tacs i) st)
-                  else
-                    (trace_tac "*** Wrong number of produced goals" THEN bailout_tac) st
-                
-              , 
-                K (trace_tac "*** Phase tactic failed" THEN bailout_tac))
-            end i st
-  
-      in
-        r phases
-      end
-
-
-    end
-
-
-    fun gen_trans_op_tac start dbg ctxt = let
-val _ = @{print} ("gen_trans_op_tac/start" ^ " " ^ 
-  (@{make_string} (Time.toMilliseconds (#elapsed (Timing.result start)))))
-      val fr_rl_net = Sepref_Translate.sepref_fr_rules.get ctxt |> Tactic.build_net
-      val fr_rl_tac = 
-        print start ctxt "fr_rl_tac/0" THEN'
-        resolve_from_net_tac ctxt fr_rl_net (* Try direct match *)
-        THEN' print start ctxt "fr_rl_tac/10"
-        ORELSE' (
-          Sepref_Frame.norm_goal_pre_tac ctxt (* Normalize precondition *) 
-        THEN' print start ctxt "fr_rl_tac/20"
-          THEN' (
-            resolve_from_net_tac ctxt fr_rl_net
-            THEN' print start ctxt "fr_rl_tac/30"
-            ORELSE' (
-              resolve_tac ctxt @{thms cons_pre_rule} (* Finally, generate a frame condition *)
-              THEN_ALL_NEW_LIST [
-                print start ctxt "fr_rl_tac/final/1" THEN'
-                SOLVED' (REPEAT_ALL_NEW_FWD (DETERM o resolve_tac ctxt @{thms CPR_TAG_rules})),
-                print start ctxt "fr_rl_tac/final/10" THEN'
-                K all_tac,  (* Frame remains unchanged as first goal, even if fr_rl creates side-conditions *)
-                print start ctxt "fr_rl_tac/final/20" THEN'
-                resolve_from_net_tac ctxt fr_rl_net
-              ]
-            )
-          )  
-        )
-      
-  (***** Side Condition Solving *)
-  local
-    open Sepref_Basic
-  in
-  
-    fun side_unfold_tac ctxt = let
-      (*val ctxt = put_simpset HOL_basic_ss ctxt
-        addsimps sepref_prep_side_simps.get ctxt*)
-    in
-      CONVERSION (Id_Op.unprotect_conv ctxt)
-      THEN' SELECT_GOAL (Local_Defs.unfold0_tac ctxt @{thms bind_ref_tag_def})
-      THEN' TRY o (hyp_subst_tac ctxt)
-      (*THEN' asm_full_simp_tac ctxt*)
-    end
-  
-    (* TODO: Not accessible as single ML function? *)
-    fun linarith_tac ctxt = 
-      Method.insert_tac ctxt (rev (Named_Theorems.get ctxt \<^named_theorems>\<open>arith\<close>))
-      THEN' Lin_Arith.tac ctxt
-    
-    fun bounds_tac ctxt = let
-      val ctxt = ctxt 
-        addSDs Named_Theorems_Rev.get ctxt @{named_theorems_rev sepref_bounds_dest}
-        addsimps Named_Theorems_Rev.get ctxt @{named_theorems_rev sepref_bounds_simps}
-    in
-      TRADE (fn ctxt => 
-        SELECT_GOAL (auto_tac ctxt)
-        THEN_ALL_NEW TRY o linarith_tac ctxt
-      ) ctxt
-    end
-    
-    fun side_fallback_tac ctxt = 
-      side_unfold_tac ctxt 
-      THEN' (
-print start ctxt "side_fallback_tac/auto" THEN'
-        TRADE (SELECT_GOAL o auto_tac) ctxt
-        THEN_ALL_NEW (print start ctxt "side_fallback_tac/auto/end" THEN' TRY o SOLVED' (bounds_tac ctxt))
-THEN' print start ctxt "side_fallback_tac/end"
-      )
-  
-    val side_frame_tac = Sepref_Frame.frame_tac side_fallback_tac
-    val side_merge_tac = Sepref_Frame.merge_tac side_fallback_tac
-    val side_free_tac = Sepref_Frame.free_tac side_fallback_tac
-    
-    
-    fun side_constraint_tac ctxt = Sepref_Constraints.constraint_tac ctxt
-    
-    val pf_mono_tac = Subgoal.FOCUS_PREMS (fn {context=ctxt,...} => CHANGED (ALLGOALS (Partial_Function.mono_tac ctxt)))
-    
-    fun side_mono_tac ctxt = side_unfold_tac ctxt THEN' TRADE pf_mono_tac ctxt
-  
-    fun side_gen_algo_tac ctxt = 
-      side_unfold_tac ctxt
-      THEN' resolve_tac ctxt (Named_Theorems_Rev.get ctxt @{named_theorems_rev sepref_gen_algo_rules})
-  
-    fun side_pref_def_tac ctxt = 
-      side_unfold_tac ctxt THEN' 
-      TRADE (fn ctxt => 
-        resolve_tac ctxt @{thms PREFER_tagI DEFER_tagI} 
-        THEN' (Sepref_Debugging.warning_tac' "Obsolete PREFER/DEFER side condition" ctxt THEN' Tagged_Solver.solve_tac ctxt)
-      ) ctxt
-
-
-    fun side_rprem_tac ctxt = 
-      resolve_tac ctxt @{thms RPREMI} THEN' Refine_Util.rprems_tac ctxt
-      THEN' (K (smash_new_rule ctxt))
-
-    (*
-      Solve side condition, or invoke hnr_tac on hn_refine goal.
-
-      In debug mode, side-condition solvers are allowed to not completely solve 
-      the side condition, but must change the goal.
-    *)  
-    fun side_cond_dispatch_tac start dbg hnr_tac ctxt = let
-      fun MK tac = if dbg then CHANGED o tac ctxt else SOLVED' (tac ctxt)
-
-      val t_merge = MK side_merge_tac
-      val t_frame = MK side_frame_tac
-      val t_free = MK side_free_tac
-      val t_indep = MK Indep_Vars.indep_tac
-      val t_constraint = MK side_constraint_tac
-      val t_mono = MK side_mono_tac
-      val t_pref_def = MK side_pref_def_tac
-      val t_rprem = MK side_rprem_tac
-      val t_gen_algo = side_gen_algo_tac ctxt
-      val t_cp_cond = MK (apply_method_noargs @{method cp_solve_cond})
-      val t_cp_simplify = MK (apply_method_noargs @{method cp_simplify})
-      
-      val t_fallback = MK side_fallback_tac
-      fun AROUND txt tac = print start ctxt ("start " ^ txt) THEN' tac THEN' print start ctxt ("end " ^ txt)
-    in
-      WITH_concl 
-        (fn @{mpat "Trueprop ?t"} => (case t of
-              @{mpat "MERGE _ _ _ _ _"} => AROUND "t_merge" t_merge
-            | @{mpat "MK_FREE _ _"} => AROUND "t_free" t_free
-            | @{mpat "_ \<turnstile> _"} => AROUND "t_frame" t_frame
-            | @{mpat "INDEP _"} => AROUND "indep" t_indep     (* TODO: Get rid of this!? *)
-            | @{mpat "CONSTRAINT _ _"} => AROUND "CONSTRAINT"  t_constraint
-            | @{mpat "M.mono_body _"} => AROUND "mono" t_mono
-            | @{mpat "PREFER_tag _"} => AROUND "pref" t_pref_def
-            | @{mpat "DEFER_tag _"} => AROUND "deref" t_pref_def
-            | @{mpat "RPREM _"} => AROUND "rprem" t_rprem
-            | @{mpat "GEN_ALGO _ _"} => AROUND "gen" t_gen_algo
-            | @{mpat "CP_cond _"} => AROUND "cond" t_cp_cond           
-            | @{mpat "CP_simplify _ _"} => AROUND "simplify" t_cp_simplify
-            | @{mpat "hn_refine _ _ _ _ _ _"} => AROUND "refine" hnr_tac 
-            | _ => AROUND "fallback" t_fallback
-          )
-        | _ => K no_tac  
-      )
-    end
-
-  end  
-      val side_tac = print start ctxt "side_tac/inner" THEN' REPEAT_ALL_NEW_FWD 
-(print start ctxt "side_tac/REPEAT_ALL_NEW_FWD" THEN' side_cond_dispatch_tac start false (K no_tac) ctxt)
-
-      val fr_tac = 
- (*        if dbg then (* Present all possibilities with (partially resolved) side conditions *)
-          fr_rl_tac THEN_ALL_NEW_FWD (TRY o side_tac)
-        else (* Choose first rule that solves all side conditions *) *)
-          DETERM o SOLVED' (print start ctxt "fr_tac" THEN' fr_rl_tac THEN_ALL_NEW_FWD (print start ctxt "side_tac" THEN' SOLVED' side_tac))
-
-    in
-      PHASES' start [
-        (fn () => "Align goal" ^ " " ^ (@{make_string} (Time.toMilliseconds (#elapsed (Timing.result start)))),Sepref_Frame.align_goal_tac, 0),
-        (fn () => "Frame rule" ^ " " ^ (@{make_string} (Time.toMilliseconds (#elapsed (Timing.result start)))),fn ctxt => resolve_tac ctxt @{thms trans_frame_rule}, 1),
-        (* RECOVER_PURE goal *)
-        (fn () => "Recover pure" ^ " " ^ (@{make_string} (Time.toMilliseconds (#elapsed (Timing.result start)))),Sepref_Frame.recover_pure_tac, ~1),
-        (* hn-refine goal with stripped precondition *)
-        (fn () => "Apply rule" ^ " " ^ (@{make_string} (Time.toMilliseconds (#elapsed (Timing.result start)))),K fr_tac,~1)
-      ] (Sepref_Basic.flag_phases_ctrl ctxt dbg) ctxt
-    end
-
-      
-fun gen_trans_step_tac start dbg ctxt = Sepref_Translate.side_cond_dispatch_tac dbg
-      ( Sepref_Frame.norm_goal_pre_tac ctxt 
-        THEN' print start ctxt "THEN'"
-        THEN' ((print start ctxt "THEN'/1 start" 
-                 THEN' Sepref_Frame.align_goal_tac ctxt
-                 THEN' print start ctxt "THEN'/1 5"
-                 THEN' Sepref_Translate.trans_comb_tac ctxt THEN' print start ctxt "THEN'/1 end")
-              ORELSE' (print start ctxt "THEN'/2 start"
-                 THEN' gen_trans_op_tac start dbg ctxt THEN' print start ctxt "THEN'/2 end")))
-      ctxt\<close>
-setup \<open>map_theory_claset (fn ctxt => ctxt delSWrapper ("split_all_tac"))\<close>
-setup \<open>map_theory_claset (fn ctxt => ctxt addSbefore ("split_all_tac", split_all_tac))\<close>
-
-  method handle_CP_SEQ =  
-    drule CP_HANDLED,
-    erule CP_SEQE,
-    (elim conjE)?,
-    (*cp_sels_to_vars?,
-    cp_vars_to_sels?,*)
-    solves cp_resolve_tag | (cp_explode_prod?, cp_resolve_tag)
 
 sepref_def decide_wl_or_skip_D_fast_code
   is \<open>decide_wl_or_skip_D_heur\<close>
   :: \<open>isasat_bounded_assn\<^sup>d \<rightarrow>\<^sub>a bool1_assn \<times>\<^sub>a isasat_bounded_assn\<close>
   supply[[goals_limit=1]]
   apply (rule hfref_refine_with_pre[OF decide_wl_or_skip_D_heur'_decide_wl_or_skip_D_heur, unfolded Down_id_eq])
-  unfolding decide_wl_or_skip_D_heur'_def
-  unfolding fold_tuple_optimizations option.case_eq_if atom.fold_option
-  apply sepref_dbg_preproc
-  apply sepref_dbg_cons_init
-  apply sepref_dbg_id
-  apply sepref_dbg_monadify
-  apply sepref_dbg_opt_init
-  apply sepref_dbg_trans_step
-  apply sepref_dbg_trans_step
-  apply sepref_dbg_trans_step
-  apply sepref_dbg_trans_step
-  apply sepref_dbg_trans_step
-  apply sepref_dbg_trans_step
-  apply sepref_dbg_trans_step
-  apply sepref_dbg_trans_step
-apply (tactic \<open> (REPEAT_DETERM_N 50 ( Sepref_Translate.trans_step_tac @{context} 1))\<close>)
-                      apply (tactic \<open> (REPEAT_DETERM_N 35 ( Sepref_Translate.trans_step_tac @{context} 1))\<close>)
-  supply [cp_solve_cond_pre] = CP_simps 
-  apply (rule CP_simplifyI)
-            apply (determ \<open>((thin_tac "_")+)?\<close>)
-            apply (rule impI)
-    apply ( (simp only: CP_simps cong: CP_tag_cong)?)
-            apply (determ \<open>cp_normalize_step\<close>)
-            apply (determ \<open>cp_normalize_step\<close>)
-               apply (determ \<open>cp_normalize_step\<close>)
-  apply (handle_CP_SEQ)
-  apply (drule CP_HANDLED,
-    erule CP_EXE)
-              apply ((elim conjE)?)
-  apply (subst (asm) prod_eq_iff)
-  apply (subst (asm) prod_eq_iff)
-  apply (subst (asm) prod_eq_iff)
-  apply (subst (asm) prod_eq_iff)
-  apply (subst (asm) prod_eq_iff)
-  apply (subst (asm) prod_eq_iff)
-  apply (subst (asm) prod_eq_iff)
-  apply (subst (asm) prod_eq_iff)
-  apply (subst (asm) prod_eq_iff)
-  apply (subst (asm) prod_eq_iff)
-  apply (subst (asm) prod_eq_iff)
-  apply (subst (asm) prod_eq_iff)
-  apply (subst (asm) prod_eq_iff)
-  apply (subst (asm) prod_eq_iff)
-  apply (subst (asm) prod_eq_iff)
-  apply (subst (asm) prod_eq_iff)
-  apply (subst (asm) prod_eq_iff)
-  apply (subst (asm) prod_eq_iff)
-  apply (subst (asm) prod_eq_iff)
-  apply (subst (asm) prod_eq_iff)
-  apply (subst (asm) prod_eq_iff)
-  apply (subst (asm) prod_eq_iff)
-  apply (subst (asm) prod_eq_iff)
-  apply (subst (asm) prod_eq_iff)
-  apply (subst (asm) prod_eq_iff)
-  apply (subst (asm) prod_eq_iff)
-  apply (subst (asm) prod_eq_iff)
-  apply (subst (asm) prod_eq_iff)
-  apply (subst (asm) prod_eq_iff)
-  apply (subst (asm) prod_eq_iff)
-  apply (subst (asm) prod_eq_iff)
-  apply (subst (asm) prod_eq_iff)
-  apply (subst (asm) prod_eq_iff)
-  apply (subst (asm) prod_eq_iff)
-  apply (subst (asm) prod_eq_iff)
-  apply (subst (asm) prod_eq_iff)
-  apply (subst (asm) prod_eq_iff)
-  apply (subst (asm) prod_eq_iff)
-              supply [[simp_trace=false]]
-               apply ((simp only: (* prod_eq_iff *)  prod.inject cnv_conj_to_meta (* fst_conv snd_conv *)  cong: CP_tag_cong))
-               apply (cp_resolve_tag)
-
-  thm prod_eq_iff
-              apply (drule CP_monos[THEN CP_HANDLEI] | handle_plain_eqs
-       |handle_CP_SEQ|handle_CP_EX(*handle_CP_EX32
-      |handle_CP_JOIN|handle_CP_RPT *)
-    
-)
-  unfolding CP_simps
-  apply (rule CP_simp_join_triv)
-  apply (tactic \<open>HEADGOAL (gen_trans_step_tac (Timing.start ()) true @{context})\<close>)
-apply (tactic \<open> (REPEAT_DETERM_N 50 ( Sepref_Translate.trans_step_tac @{context} 1))\<close>)
-  oops
-apply (tactic \<open> (REPEAT_DETERM_N 1 ( Sepref_Translate.trans_step_tac @{context} 1))\<close>)
-(*
-supply [[simp_trace]]
-apply sepref_dbg_trans_step
-  *)
-  oops
-apply (tactic \<open> (REPEAT_DETERM_N 1 ( Sepref_Translate.trans_step_tac @{context} 1))\<close>)
-oops
-  ML \<open>Sepref_Translate.trans_step_tac\<close>
-  apply sepref_dbg_opt
-  apply sepref_dbg_cons_solve
-  apply sepref_dbg_cons_solve
-  apply sepref_dbg_cons_solve_cp
-  apply sepref_dbg_constraints
+  unfolding decide_wl_or_skip_D_heur'_def option.case_eq_if atom.fold_option
   by sepref
-
 
 experiment begin
 
